DbAppProgramLogic/Basic.lean
@@ -1,4 +1,6 @@
 import DbAppProgramLogic.Syntax
 import DbAppProgramLogic.Semantics
+import DbAppProgramLogic.SetLanguage
 import DbAppProgramLogic.Logic
 import DbAppProgramLogic.Transformer
+import DbAppProgramLogic.Examples
